rename

src/lib/data/Kuiper.ArrayView.fst
@@ -7,14 +7,14 @@ module B = Kuiper.Array (* base *)
 module T = FStar.Tactics.V2
 module SZ = FStar.SizeT
 
-let gpu_array #a #len #vt vw =
-  Kuiper.Array.gpu_array a len
+let varray #a #len #vt vw =
+  B.gpu_array a len
 
 let core a = a
 
-let gpu_array_pts_to
+let varray_pts_to
   (#et:Type) (#len : erased nat) (#vt:_) (#vw : aview et len vt)
-  ([@@@mkey] a : gpu_array vw)
+  ([@@@mkey] a : varray vw)
   (#[T.exact (`1.0R)] f : perm)
   (v : vt)
   : slprop
@@ -22,45 +22,45 @@ let gpu_array_pts_to
     B.gpu_pts_to_array a #f (vw.bij.gg v)
 
 inline_for_extraction noextract
-fn gpu_array_concr
+fn varray_concr
   (#t:Type0)
   (#len : erased nat)
   (#vt:Type0)
   (#vw : aview t len vt)
-  (a : gpu_array vw)
+  (a : varray vw)
   (#v : vt)
   requires
     a |-> v
   ensures
     core a |-> vw.bij.gg v
 {
-  unfold gpu_array_pts_to a v;
+  unfold varray_pts_to a v;
 }
 
 inline_for_extraction noextract
-fn gpu_array_abs
+fn varray_abs
   (#t:Type0)
   (#len0 : erased nat) (#vt0:Type0) (#vw0 : aview t len0 vt0)
-  (a : gpu_array vw0)
+  (a : varray vw0)
   (#len : erased nat) (#vt:Type0) (vw : aview t len vt)
   (#v : vt)
   requires
     core a |-> vw.bij.gg v
   returns
-    a' : gpu_array vw
+    a' : varray vw
   ensures
     pure (len0 == len /\ core a == core a') **
     (a' |-> v)
 {
   gpu_pts_to_ref (core a);
-  let a' : gpu_array vw = core a;
+  let a' : varray vw = core a;
   rewrite each core a as a';
-  fold gpu_array_pts_to #t #len #vt #vw a' #1.0R v;
+  fold varray_pts_to #t #len #vt #vw a' #1.0R v;
   a'
 }
 
 inline_for_extraction noextract
-fn gpu_array_alloc0
+fn varray_alloc0
   (#et:Type) {| sized et |}
   (len : SZ.t) (#vt:Type0) (vw : aview et len vt)
   preserves
@@ -68,7 +68,7 @@ fn gpu_array_alloc0
   requires
     pure (SZ.fits len)
   returns
-    a : gpu_array vw
+    a : varray vw
   ensures
     exists* v. a |-> v
 {
@@ -76,12 +76,12 @@ fn gpu_array_alloc0
   with v.
     assert (a |-> v);
   rewrite each v as vw.bij.gg (vw.bij.ff v);
-  fold gpu_array_pts_to #et #len #vt #vw a #1.0R (vw.bij.ff v);
+  fold varray_pts_to #et #len #vt #vw a #1.0R (vw.bij.ff v);
   a
 }
 
 // inline_for_extraction noextract
-// fn gpu_array_alloc1
+// fn varray_alloc1
 //   (#et:Type) {| sized et |}
 //   (#len : SZ.t) (#vt:Type0) (vw : aview et len vt)
 //   (v0 : vt)
@@ -90,20 +90,20 @@ fn gpu_array_alloc0
 //   requires
 //     pure (SZ.fits len)
 //   returns
-//     a : gpu_array vw
+//     a : varray vw
 //   ensures
 //     a |-> v0
 // {
-//   let a = gpu_array_alloc0 #et len vw;
+//   let a = varray_alloc0 #et len vw;
 //   (* fill? *)
 //   admit();
 // }
 
 inline_for_extraction noextract
-fn gpu_array_free
+fn varray_free
   (#et:Type) {| sized et |}
   (#len : erased nat) (#vt:Type0) (vw : aview et len vt)
-  (a : gpu_array vw)
+  (a : varray vw)
   (#v : vt)
   preserves
     cpu
@@ -111,100 +111,100 @@ fn gpu_array_free
     a |-> v
   ensures emp
 {
-  unfold gpu_array_pts_to a v;
+  unfold varray_pts_to a v;
   B.gpu_array_free a;
 }
 
 ghost
-fn gpu_array_share_n
+fn varray_share_n
   (#et:Type)
   (#len : erased nat) (#vt:Type0) (vw : aview et len vt)
   (#[T.exact (`0)] uid: int)
-  (a : gpu_array vw)
+  (a : varray vw)
   (k : pos)
   (#f : perm)
   (#v : vt)
   requires
-    gpu_array_pts_to a #f v
+    varray_pts_to a #f v
   ensures
-    bigstar #uid 0 k (fun _ -> gpu_array_pts_to a #(f /. k) v)
+    bigstar #uid 0 k (fun _ -> varray_pts_to a #(f /. k) v)
 {
-  unfold gpu_array_pts_to a #f v;
+  unfold varray_pts_to a #f v;
   B.gpu_slice_share #uid a 0 len k;
 }
 
 ghost
-fn gpu_array_gather_n
+fn varray_gather_n
   (#et:Type)
   (#len : erased nat) (#vt:Type0) (vw : aview et len vt)
   (#uid: int)
-  (a : gpu_array vw)
+  (a : varray vw)
   (k : pos)
   (#f : perm)
   (#v : vt)
   requires
-    bigstar #uid 0 k (fun _ -> gpu_array_pts_to a #(f /. k) v)
+    bigstar #uid 0 k (fun _ -> varray_pts_to a #(f /. k) v)
   ensures
-    gpu_array_pts_to a #f v
+    varray_pts_to a #f v
 {
   B.gpu_slice_gather #uid a 0 len k;
-  fold gpu_array_pts_to a #f v;
+  fold varray_pts_to a #f v;
 }
 
 inline_for_extraction noextract
-fn gpu_array_read
+fn varray_read
   (#et:Type)
   (#len : erased nat) (#vt:Type0) (vw : aview et len vt)
-  (a : gpu_array vw)
+  (a : varray vw)
   (i : vw.it)
   (#f : perm)
   (#v : vt)
   requires
     gpu **
-    gpu_array_pts_to a #f v
+    varray_pts_to a #f v
   returns
     e : et
   ensures
     gpu **
-    gpu_array_pts_to a #f v **
+    varray_pts_to a #f v **
     pure (e == vw.acc i v)
 {
   let ci = cidx vw i;
-  unfold gpu_array_pts_to a #f v;
+  unfold varray_pts_to a #f v;
   let r = B.gpu_array_read #et #len #0 #len a #f ci;
   vw.galois1 v i;
-  fold gpu_array_pts_to a #f v;
+  fold varray_pts_to a #f v;
   r
 }
 
 inline_for_extraction noextract
-fn gpu_array_write
+fn varray_write
   (#et:Type)
   (#len : erased nat) (#vt:Type0) (vw : aview et len vt)
-  (a : gpu_array vw)
+  (a : varray vw)
   (i : vw.it)
   (e : et)
   (#f : perm)
   (#v0 : vt)
   requires
     gpu **
-    gpu_array_pts_to a v0
+    varray_pts_to a v0
   ensures
     gpu **
-    gpu_array_pts_to a (vw.upd i e v0)
+    varray_pts_to a (vw.upd i e v0)
 {
   let ci = cidx vw i;
-  unfold gpu_array_pts_to a v0;
+  unfold varray_pts_to a v0;
   B.gpu_array_write #et #len #0 #len a ci e;
   vw.galois2 v0 i e;
-  fold gpu_array_pts_to a (vw.upd i e v0);
+  fold varray_pts_to a (vw.upd i e v0);
   ()
 }
 
-let gpu_array_pts_to_cell
+let varray_pts_to_cell
   (#et:Type)
   (#len : erased nat) (#vt:Type0) (#vw : aview et len vt)
-  ([@@@mkey] a : gpu_array vw)
+  ([@@@mkey] a : varray vw)
   (#[T.exact (`1.0R)] f : perm)
   ([@@@mkey]i : vw.it)
   (v : et)
@@ -212,69 +212,69 @@ let gpu_array_pts_to_cell
   = gpu_pts_to_slice a #f (vw.ibij.gg i) (vw.ibij.gg i + 1) seq![v]
 
 inline_for_extraction noextract
-fn gpu_array_read_cell
+fn varray_read_cell
   (#et:Type)
   (#len : erased nat) (#vt:Type0) (vw : aview et len vt)
-  (a : gpu_array vw)
+  (a : varray vw)
   (i : vw.it)
   (#f : perm)
   (#v0 : erased et)
   requires
     gpu **
-    gpu_array_pts_to_cell a #f i v0
+    varray_pts_to_cell a #f i v0
   returns
     v : et
   ensures
     gpu **
-    gpu_array_pts_to_cell a #f i v **
+    varray_pts_to_cell a #f i v **
     pure (v == v0)
 {
   let ci = cidx vw i;
-  unfold gpu_array_pts_to_cell a #f i v0;
+  unfold varray_pts_to_cell a #f i v0;
   let r = B.gpu_array_read #et #len #ci #(ci+1) a #f ci;
-  fold gpu_array_pts_to_cell a #f i v0;
+  fold varray_pts_to_cell a #f i v0;
   r
 }
 
 inline_for_extraction noextract
-fn gpu_array_write_cell
+fn varray_write_cell
   (#et:Type)
   (#len : erased nat) (#vt:Type0) (vw : aview et len vt)
-  (a : gpu_array vw)
+  (a : varray vw)
   (i : vw.it)
   (v1 : et)
   (#v0 : erased et)
   requires
     gpu **
-    gpu_array_pts_to_cell a i v0
+    varray_pts_to_cell a i v0
   ensures
     gpu **
-    gpu_array_pts_to_cell a i v1
+    varray_pts_to_cell a i v1
 {
   let ci = cidx vw i;
-  unfold gpu_array_pts_to_cell a i v0;
+  unfold varray_pts_to_cell a i v0;
   B.gpu_array_write #_ #_ #ci #(ci+1) a ci v1;
   with s'. assert (B.gpu_pts_to_slice a ci (ci+1) s');
   Kuiper.Seq.Common.lem_one_elem s' v1;
-  fold gpu_array_pts_to_cell a i v1;
+  fold varray_pts_to_cell a i v1;
   ()
 }
 
 ghost
-fn gpu_array_explode
+fn varray_explode
   (#et:Type)
   (#len : erased nat) (#vt:Type0) (vw : aview et len vt)
-  (a : gpu_array vw)
+  (a : varray vw)
   (#f : perm)
   (#v : vt)
   requires
-    gpu_array_pts_to a #f v
+    varray_pts_to a #f v
   ensures
     forall+ (i : vw.it).
-      gpu_array_pts_to_cell #et #len #vt #vw a #f i (vw.acc i v)
+      varray_pts_to_cell #et #len #vt #vw a #f i (vw.acc i v)
 {
-  unfold gpu_array_pts_to a #f v;
-  gpu_array_slice_1 a;
+  unfold varray_pts_to a #f v;
+  B.gpu_array_slice_1 a;
   rewrite
     bigstar 0 len
      (fun i -> gpu_pts_to_slice a #f i (i+1) seq![vw.bij.gg v @! i])
@@ -295,17 +295,17 @@ fn gpu_array_explode
 }
 
 ghost
-fn gpu_array_implode
+fn varray_implode
   (#et:Type)
   (#len : erased nat) (#vt:Type0) (vw : aview et len vt)
-  (a : gpu_array vw)
+  (a : varray vw)
   (#f : perm)
   (#v : vt)
   requires
     forall+ (i : vw.it).
-      gpu_array_pts_to_cell #et #len #vt #vw a #f i (vw.acc i v)
+      varray_pts_to_cell #et #len #vt #vw a #f i (vw.acc i v)
   ensures
-    gpu_array_pts_to a #f v
+    varray_pts_to a #f v
 {
   Classical.forall_intro_2 vw.galois1;
   forevery_ext #vw.it
@@ -315,6 +315,6 @@ fn gpu_array_implode
       (fun i -> gpu_pts_to_slice a #f i (i+1) seq![vw.bij.gg v @! i]);
   forevery_tostar #(natlt len)
       (fun i -> gpu_pts_to_slice a #f i (i+1) seq![vw.bij.gg v @! i]);
-  gpu_array_unslice_1 a;
-  fold gpu_array_pts_to a #f v;
+  B.gpu_array_unslice_1 a;
+  fold varray_pts_to a #f v;
 }
