src/lib/data/Kuiper.ArrayView.fsti
@@ -40,36 +40,36 @@ let cidx (#a : Type) (#len : erased nat) (#vt : Type)
 // type mrepr = #len:nat -> alayout a len vt rows
 
 inline_for_extraction noextract
-val gpu_array (#a : Type0) (#len : nat) (#vt : Type) (vw : aview a len vt) : Type0
+val varray (#a : Type0) (#len : nat) (#vt : Type) (vw : aview a len vt) : Type0
 
 inline_for_extraction noextract
 val core
   (#a : Type)
   (#len : erased nat)
   (#vt : Type) (#vw : aview a len vt)
-  (g : gpu_array vw)
+  (g : varray vw)
   : Kuiper.Array.gpu_array a len
 
-val gpu_array_pts_to
+val varray_pts_to
   (#a:Type) (#len : erased nat) (#vt:_) (#vw : aview a len vt)
-  ([@@@mkey] a : gpu_array vw)
+  ([@@@mkey] a : varray vw)
   (#[T.exact (`1.0R)] f : perm)
   (v : vt)
   : slprop
 
 unfold
 instance has_pts_to (#a:Type) (#len : nat) (#vt:Type) (#vw : aview a len vt)
-  : has_pts_to (gpu_array vw) vt = {
-  pts_to = gpu_array_pts_to;
+  : has_pts_to (varray vw) vt = {
+  pts_to = varray_pts_to;
 }
 
 inline_for_extraction noextract
-fn gpu_array_concr
+fn varray_concr
   (#t:Type0)
   (#len : erased nat)
   (#vt:Type0)
   (#vw : aview t len vt)
-  (a : gpu_array vw)
+  (a : varray vw)
   (#v : vt)
   requires
     a |-> v
@@ -77,22 +77,22 @@ fn gpu_array_concr
     core a |-> vw.bij.gg v
 
 inline_for_extraction noextract
-fn gpu_array_abs
+fn varray_abs
   (#t:Type0)
   (#len0 : erased nat) (#vt0:Type0) (#vw0 : aview t len0 vt0)
-  (a : gpu_array vw0)
+  (a : varray vw0)
   (#len : erased nat) (#vt:Type0) (vw : aview t len vt)
   (#v : vt)
   requires
     core a |-> vw.bij.gg v
   returns
-    a' : gpu_array vw
+    a' : varray vw
   ensures
     pure (len0 == len /\ core a == core a') **
     (a' |-> v)
 
 inline_for_extraction noextract
-fn gpu_array_alloc0
+fn varray_alloc0
   (#et:Type) {| sized et |}
   (len : SZ.t) (#vt:Type0) (vw : aview et len vt)
   preserves
@@ -100,15 +100,15 @@ fn gpu_array_alloc0
   requires
     pure (SZ.fits len)
   returns
-    a : gpu_array vw
+    a : varray vw
   ensures
     exists* v. a |-> v
 
 inline_for_extraction noextract
-fn gpu_array_free
+fn varray_free
   (#et:Type) {| sized et |}
   (#len : erased nat) (#vt:Type0) (vw : aview et len vt)
-  (a : gpu_array vw)
+  (a : varray vw)
   (#v : vt)
   preserves
     cpu
@@ -117,72 +117,72 @@ fn gpu_array_free
   ensures emp
 
 ghost
-fn gpu_array_share_n
+fn varray_share_n
   (#et:Type)
   (#len : erased nat) (#vt:Type0) (vw : aview et len vt)
   (#[T.exact (`0)] uid: int)
-  (a : gpu_array vw)
+  (a : varray vw)
   (k : pos)
   (#f : perm)
   (#v : vt)
   requires
-    gpu_array_pts_to a #f v
+    varray_pts_to a #f v
   ensures
-    bigstar #uid 0 k (fun _ -> gpu_array_pts_to a #(f /. k) v)
+    bigstar #uid 0 k (fun _ -> varray_pts_to a #(f /. k) v)
 
 ghost
-fn gpu_array_gather_n
+fn varray_gather_n
   (#et:Type)
   (#len : erased nat) (#vt:Type0) (vw : aview et len vt)
   (#uid: int)
-  (a : gpu_array vw)
+  (a : varray vw)
   (k : pos)
   (#f : perm)
   (#v : vt)
   requires
-    bigstar #uid 0 k (fun _ -> gpu_array_pts_to a #(f /. k) v)
+    bigstar #uid 0 k (fun _ -> varray_pts_to a #(f /. k) v)
   ensures
-    gpu_array_pts_to a #f v
+    varray_pts_to a #f v
 
 inline_for_extraction noextract
-fn gpu_array_read
+fn varray_read
   (#et:Type)
   (#len : erased nat) (#vt:Type0) (vw : aview et len vt)
-  (a : gpu_array vw)
+  (a : varray vw)
   (i : vw.it)
   (#f : perm)
   (#v : vt)
   requires
     gpu **
-    gpu_array_pts_to a #f v
+    varray_pts_to a #f v
   returns
     e : et
   ensures
     gpu **
-    gpu_array_pts_to a #f v **
+    varray_pts_to a #f v **
     pure (e == vw.acc i v)
 
 inline_for_extraction noextract
-fn gpu_array_write
+fn varray_write
   (#et:Type)
   (#len : erased nat) (#vt:Type0) (vw : aview et len vt)
-  (a : gpu_array vw)
+  (a : varray vw)
   (i : vw.it)
   (e : et)
   (#f : perm)
   (#v0 : vt)
   requires
     gpu **
-    gpu_array_pts_to a v0
+    varray_pts_to a v0
   ensures
     gpu **
-    gpu_array_pts_to a (vw.upd i e v0)
+    varray_pts_to a (vw.upd i e v0)
 
 (* Ownership over a single index. *)
-val gpu_array_pts_to_cell
+val varray_pts_to_cell
   (#et:Type)
   (#len : erased nat) (#vt:Type0) (#vw : aview et len vt)
-  ([@@@mkey] a : gpu_array vw)
+  ([@@@mkey] a : varray vw)
   (#[T.exact (`1.0R)] f : perm)
   ([@@@mkey]i : vw.it)
   (v : et)
@@ -191,60 +191,60 @@ val gpu_array_pts_to_cell
 (* Ownership over a single index. *)
 
 inline_for_extraction noextract
-fn gpu_array_read_cell
+fn varray_read_cell
   (#et:Type)
   (#len : erased nat) (#vt:Type0) (vw : aview et len vt)
-  (a : gpu_array vw)
+  (a : varray vw)
   (i : vw.it)
   (#f : perm)
   (#v0 : erased et)
   requires
     gpu **
-    gpu_array_pts_to_cell a #f i v0
+    varray_pts_to_cell a #f i v0
   returns
     v : et
   ensures
     gpu **
-    gpu_array_pts_to_cell a #f i v **
+    varray_pts_to_cell a #f i v **
     pure (v == v0)
 
 inline_for_extraction noextract
-fn gpu_array_write_cell
+fn varray_write_cell
   (#et:Type)
   (#len : erased nat) (#vt:Type0) (vw : aview et len vt)
-  (a : gpu_array vw)
+  (a : varray vw)
   (i : vw.it)
   (v1 : et)
   (#v0 : erased et)
   requires
     gpu **
-    gpu_array_pts_to_cell a i v0
+    varray_pts_to_cell a i v0
   ensures
     gpu **
-    gpu_array_pts_to_cell a i v1
+    varray_pts_to_cell a i v1
 
 ghost
-fn gpu_array_explode
+fn varray_explode
   (#et:Type)
   (#len : erased nat) (#vt:Type0) (vw : aview et len vt)
-  (a : gpu_array vw)
+  (a : varray vw)
   (#f : perm)
   (#v : vt)
   requires
-    gpu_array_pts_to a #f v
+    varray_pts_to a #f v
   ensures
     forall+ (i : vw.it).
-      gpu_array_pts_to_cell #et #len #vt #vw a #f i (vw.acc i v)
+      varray_pts_to_cell #et #len #vt #vw a #f i (vw.acc i v)
 
 ghost
-fn gpu_array_implode
+fn varray_implode
   (#et:Type)
   (#len : erased nat) (#vt:Type0) (vw : aview et len vt)
-  (a : gpu_array vw)
+  (a : varray vw)
   (#f : perm)
   (#v : vt)
   requires
     forall+ (i : vw.it).
-      gpu_array_pts_to_cell #et #len #vt #vw a #f i (vw.acc i v)
+      varray_pts_to_cell #et #len #vt #vw a #f i (vw.acc i v)
   ensures
-    gpu_array_pts_to a #f v
+    varray_pts_to a #f v
